modified:   coq/div2.v 	modified:   coq/sort.v 	new file:   coq/testor.v 	new file:   haskell/Barcode.hs 	modified:   haskell/QC.hs 	new file:   js/bitcoinj-core-0.14.2-bundled.jar 	new file:   js/bitcoinj.js 	new file:   js/demo.js 	modified:   polyglot/Interpreter/Interpreter.java 	new file:   polyglot/Interpreter/Interpreter.scala 	new file:   polyglot/Interpreter/interpreter.cs 	modified:   polyglot/Interpreter/run.sh 	modified:   polyglot/Interpreter/search.sh 	modified:   scm/evaluator/TODO 	modified:   scm/evaluator/analyze.scm 	modified:   scm/evaluator/defined.scm 	modified:   scm/evaluator/eval.scm 	modified:   scm/evaluator/if.scm 	modified:   scm/evaluator/lambda.scm 	modified:   scm/evaluator/not.scm

haskell/Barcode.hs
@@ -1,0 +1,6 @@
+
+
+mapEveryOther :: (a -> a) -> [a] -> [a]
+mapEveryOther f = zipWith ($) (cycle [f,id])
+
+test0 = mapEveryOther (\x -> x * x) [2,3,4,5,6,7,8,9,10]  -- [4,3,16,5,36,7,64,9,100]
