js/demo.js
@@ -1,0 +1,13 @@
+// import some stuff
+var bcj = org.bitcoinj;
+var ECKey = bcj.core.ECKey;
+
+
+// We'll use the tesnet for now
+var params  = bcj.params.TestNet3Params.get();
+var key = new ECKey();
+
+print(key);
+
+
+
