polyglot/Interpreter/interpreter.cs
@@ -1,0 +1,158 @@
+// Interpreter Design Pattern
+using System;
+using System.Collections.Generic;
+// from the Gang of Four book:
+// "If a particular kind of problem occurs often enough, then it might be
+// worthwhile to express instances of the problem as sentences in a simple
+// language. Then you can build an interpreter that solves the problem by 
+// interpreting these sentences. For example, searching for strings that 
+// match a pattern is a common problem. Regular expressions are a standard 
+// language for specifying patterns of strings. Rather than building custom 
+// algorithms to match each pattern against strings, search algorithms could 
+// interpret a regular expression that specifies a set of strings to match."
+
+// Each regular expression r has an associated language L(r) (which is a set
+// of strings) defined by the recursion:
+//
+//  - r = Lit(s)        -> L(r) = {s}
+//  - r = And(r1, r2)   -> L(r) = L(r1).L(r2)     (see definition of '.')
+//  - r = Or(r1, r2)    -> L(r) = L(r1) U L(r2)
+//  - r = Many(r1)      -> L(r) = U_k L(r1)^k     (see definition of '.')
+//
+//  where given A,B sets of strings the product A.B is defined as the set of 
+//  strings A.B = { a ++ b | a in A, b in B }, and where it is understood that
+//  A^0 = {""} and A^1 = A. 
+//
+// Given a regular expression r and a string s, many reasonable questions 
+// can be asked in relation to r and s. When using the command 'grep', the
+// question being asked is whether there exist a substring s' of s which
+// belongs to the language of r. One of the first questions of interest is
+// of course whether s itself belongs to L(r).
+
+abstract class Exp {
+  // static factory methods
+  public static Exp Lit(string literal){ return new Lit(literal); }
+  public static Exp And(Exp left, Exp right){ return new And(left, right); }
+  public static Exp Or(Exp left, Exp right){ return new Or(left, right); }
+  public static Exp Many(Exp regex){ return new Many(regex); }
+  // instance interface
+  public abstract override string ToString();
+  // Given a string, this method returns 'the' list of all prefixes of the string
+  // which belong to the language of the regular expression object. Of course,
+  // such a list is only unique up to the order of its elements
+  public abstract IList<string> Interpret(string input);
+  public bool Recognize(string input){ 
+    return this.Interpret(input).Contains(input);
+  }
+}
+
+class Lit : Exp {
+  private readonly string literal;
+  public Lit(string literal){ this.literal = literal; }
+  public override string ToString(){ return literal; }
+  public override IList<string> Interpret(string input){
+    IList<string> result = new List<string>();
+    if(input.StartsWith(literal)){  // literal is a prefix of input
+      result.Add(literal);
+    }
+    return result;
+  }
+}
+
+class And : Exp {
+  private readonly Exp left;
+  private readonly Exp right;
+  public And(Exp left, Exp right){ this.left = left; this.right = right; }
+  public override string ToString(){ return "" + left + right; }
+  public override IList<string> Interpret(string input){
+    IList<string> result = new List<string>();
+    IList<string> leftList = left.Interpret(input);
+    foreach(string s1 in leftList){
+      string remainder = input.Substring(s1.Length);
+      IList<string> rightList = right.Interpret(remainder);
+      foreach(string s2 in rightList){
+        result.Add(s1 + s2);
+      }
+    }
+    return result;
+  }
+}
+
+class Or  : Exp {
+  private readonly Exp left;
+  private readonly Exp right;
+  public Or(Exp left, Exp right){ this.left = left; this.right = right; }
+  public override string ToString(){ return "(" + left + "|" + right + ")" ; }
+  public override IList<string> Interpret(string input){
+    IList<string> result = left.Interpret(input);
+    IList<string> rightList = right.Interpret(input);
+    foreach(string s in rightList){
+      result.Add(s);
+    }
+    return result;
+  }
+}
+
+
+class Many: Exp{
+  private readonly Exp regex;
+  public Many(Exp regex){ this.regex = regex; }
+  public override string ToString(){ return "(" + regex + ")*"; }
+  public override IList<string> Interpret(string input){
+    IList<string> result = new List<string>();
+    result.Add(""); // forall r:Exp, "" belongs to L(r*)
+    IList<string> leftList = regex.Interpret(input);
+    foreach(string s1 in leftList){
+      if(!s1.Equals(String.Empty)){
+        string remainder = input.Substring(s1.Length);
+        IList<string> rightList = this.Interpret(remainder);  // recursive call
+        foreach(string s2 in rightList){
+          result.Add(s1 + s2);
+        }
+      }
+    }
+    return result;
+  }
+}
+
+
+public class Interpreter {
+  public static void Main(string[] args){
+    Exp a = Exp.Lit("a");
+    Exp b = Exp.Lit("b");
+    Exp c = Exp.Lit("c");
+
+    Exp aa = Exp.And(a, Exp.Many(a)); // one or more 'a'
+    Exp bb = Exp.And(b, Exp.Many(b)); // one or more 'b'
+    Exp cc = Exp.And(c, Exp.Many(c)); // one or more 'c'
+
+    Exp regex = Exp.Many(Exp.And(Exp.Or(aa,bb),cc));
+    string str = "acbbccaaacccbbbbaaaaaccccc";
+    
+    Console.WriteLine("regex = " + regex);
+    Console.WriteLine("string = \"" + str + "\"");
+    Console.WriteLine("The recognized prefixes are:");
+    IList<string> result = new List<string>();
+    for(int i = 0; i <= str.Length; ++i){
+      string test = str.Substring(0,i);
+      if(regex.Recognize(test)){
+        result.Add("\"" + test + "\"");
+      }
+    }
+    Print(result);
+  }
+
+  public static void Print(IList<string> list){
+    bool start = true;
+    Console.Write("[");
+    foreach(string s in list){
+      if(start){
+        start = false;
+      } else {
+        Console.Write(", ");
+      }
+      Console.Write(s);
+    }
+    Console.WriteLine("]");
+  }
+}
