scm/evaluator/if.scm
@@ -7,28 +7,26 @@
 
 (load "true-false.scm")
 
+; destructuring
 (define (if-predicate exp) (cadr exp))
-
 (define (if-consequent exp) (caddr exp))
-
 (define (if-alternative exp) 
-  (if (not (null? (cdddr exp)))
-    (cadddr exp)
-    '#f)) ; returning expression '#f, not the value #f
+  (if (not (null? (cdddr exp))) (cadddr exp) #f))
 
+; eval
 (define (eval-if exp env)
-  (if (true? (eval (if-predicate exp) env))                     
-    (eval (if-consequent exp) env)                             
-    (eval (if-alternative exp) env)))                          
+  (let ((pred (eval (if-predicate exp) env)))
+    (if (true? pred)
+      (eval (if-consequent exp) env)
+      (eval (if-alternative exp) env))))
 
-; added for analyze
+; analyze
 (define (analyze-if exp)
-  (let ((pproc (analyze (if-predicate exp)))
-        (cproc (analyze (if-consequent exp)))
-        (aproc (analyze (if-alternative exp))))
+  (let ((pred   (analyze (if-predicate exp)))
+        (conseq (analyze (if-consequent exp)))
+        (alter  (analyze (if-alternative exp))))
     (lambda (env)
-      (if (true? (pproc env)) (cproc env) (aproc env)))))
-
+      (if (true? (pred env)) (conseq env) (alter env)))))
 
 
 ))  ; include guard
