scm/evaluator/not.scm
@@ -7,16 +7,19 @@
 
 (load "true-false.scm")
 
+; destructuring
 (define (not-predicate exp) (cadr exp))
 
+; eval
 (define (eval-not exp env)
-  (if (true? (eval (not-predicate exp) env)) #f #t))  
+  (let ((pred (eval (not-predicate exp) env)))
+    (if (true? pred) #f #t)))  
 
-; added for analyze
+; analyze
 (define (analyze-not exp)
-  (let ((pproc (analyze (not-predicate exp))))
+  (let ((pred (analyze (not-predicate exp))))
     (lambda (env)
-      (if (true? (pproc env)) #f #t))))
+      (if (true? (pred env)) #f #t))))
 
 ))  ; include guard
 
