coq/div2.v
@@ -8,7 +8,7 @@ Fixpoint div2 (n:nat) : nat :=
   end.
 
 
-Lemma div2_le' : forall (n k:nat),
+Lemma div2_le_lem : forall (n k:nat),
   k <= n -> div2 k <= k.
 Proof.
   intros n. elim n.
@@ -26,7 +26,63 @@ Proof.
 Qed.
 
 
-Theorem div2_le: forall (n:nat), div2 n <= n.
+Theorem div2_le': forall (n:nat), div2 n <= n.
 Proof.
-  intros n. apply div2_le' with (n:=n). auto.  
+  intros n. apply div2_le_lem with (n:=n). auto.  
 Qed.
+
+
+Theorem div2_le : forall (n:nat), div2 n <= n.
+Proof.
+  intros n. cut (div2 n <= n /\ div2 (S n) <= S n). tauto.
+  elim n. simpl. auto.
+  clear n. intros n [H1 H2]. (* tick to split conjunction immediately *)
+  split. exact H2. simpl. auto with arith.
+Qed.
+
+
+Fixpoint div3 (n:nat) : nat :=
+  match n with
+    | 0           => 0
+    | 1           => 0
+    | 2           => 0
+    | S (S (S p)) => S (div3 p) 
+  end.
+
+Theorem div3_le : forall (n:nat), div3 n <= n.
+Proof.
+  intros n.
+  cut (div3 n <= n /\ div3 (S n) <= S n /\ div3 (S (S n)) <= S (S n)). tauto.
+  elim n. simpl. auto.
+  clear n. intros n [H0 [H1 H2]]. (* even bigger trick *)
+  split. exact H1. split. exact H2. simpl. auto with arith.
+Qed.
+
+
+Fixpoint mod2 (n:nat) : nat :=
+  match n with
+    | 0       => 0
+    | 1       => 1
+    | S (S p) => mod2 p
+  end.
+
+Theorem eucl2 : forall (n:nat),
+  n = 2 * (div2 n) + mod2 n.
+Proof.
+  intro n.
+  cut (n = 2 * (div2 n) + mod2 n /\ S n = 2 * (div2 (S n)) + mod2 (S n)). tauto.
+  elim n. simpl. auto.
+  clear n. intros n [H0 H1]. (* trick *)
+  split.  exact H1. simpl. rewrite plus_0_r.
+  cut (S n = div2 n + S (div2 n) + mod2 n). eauto.
+  rewrite H0 at 1. simpl. rewrite plus_0_r. simpl. 
+  rewrite <- plus_n_Sm.
+  rewrite plus_Snm_nSm.
+  rewrite <- plus_n_Sm.
+  reflexivity.
+Qed.
+
+
+
+
+
