coq/testor.v
@@ -1,0 +1,3 @@
+Inductive testor :=
+  | Constr1 : list testor -> testor
+  | Constr2 : testor -> testor.
