polyglot/Interpreter/run.sh
@@ -10,4 +10,13 @@ DIFF=$(( $END - $START ))
 echo "It took $(( $DIFF / 1000000 )) ms"
 rm *.class
 
+echo '\nThis is C# ...'
+mcs interpreter.cs 
+START=$(date +%s%N)
+mono interpreter.exe 
+END=$(date +%s%N)
+DIFF=$(( $END - $START ))
+echo "It took $(( $DIFF / 1000000 )) ms"
+rm interpreter.exe
+
 
